NuPrim.thy
@@ -223,7 +223,7 @@ subsubsection \<open>Rudimentary lemmata\<close>
 
 lemma Refining_ex: "p \<nuLinkL> R \<nuLinkR> x \<equiv> R p x" unfolding RepSet_def by simp
 lemma inhabited[dest]: "p \<nuLinkL> N \<nuLinkR> x \<Longrightarrow> x \<ratio> N" unfolding Inhabited_def by auto
-lemma [elim,\<nu>elim]: "Inhabited (U \<times> V) \<Longrightarrow> (Inhabited U \<Longrightarrow> Inhabited V \<Longrightarrow> PROP C) \<Longrightarrow> PROP C" unfolding Inhabited_def by auto
+lemma [elim!,\<nu>elim]: "Inhabited (U \<times> V) \<Longrightarrow> (Inhabited U \<Longrightarrow> Inhabited V \<Longrightarrow> PROP C) \<Longrightarrow> PROP C" unfolding Inhabited_def by auto
 lemma [intro]: "x \<in> S \<Longrightarrow> Inhabited S" unfolding Inhabited_def by auto
 lemma Inhabited_E: "Inhabited S \<Longrightarrow> (\<And>x. x \<in> S \<Longrightarrow> C) \<Longrightarrow> C" unfolding Inhabited_def by auto
 
@@ -282,7 +282,7 @@ lemma ParamTag: "\<^bold>p\<^bold>a\<^bold>r\<^bold>a\<^bold>m x" for x :: "'a" 
   \<comment>\<open>A tag used to indicate a parameter should be specified during application. It retains the order of the parameters to be specified.
   For example, "@{prop "\<And>bit_width value. \<^bold>p\<^bold>a\<^bold>r\<^bold>a\<^bold>m bit_width \<Longrightarrow> \<^bold>p\<^bold>a\<^bold>r\<^bold>a\<^bold>m value \<Longrightarrow> P bit_wdith value"},
     the first parameter `?bit_width` will be specified first and then the "?value".\<close>
-lemma [elim,\<nu>elim]: "\<^bold>p\<^bold>a\<^bold>r\<^bold>a\<^bold>m x \<Longrightarrow> C \<Longrightarrow> C" by auto
+lemma [elim!,\<nu>elim]: "\<^bold>p\<^bold>a\<^bold>r\<^bold>a\<^bold>m x \<Longrightarrow> C \<Longrightarrow> C" by auto
 
 definition ParamHOL :: " 'a \<Rightarrow> bool" where "ParamHOL x = True"
 lemma ParamHOL: "Trueprop (ParamHOL x) \<equiv> \<^bold>p\<^bold>a\<^bold>r\<^bold>a\<^bold>m x" unfolding ParamTag_def ParamHOL_def .
@@ -293,7 +293,7 @@ definition Premise :: "bool \<Rightarrow> prop" ("\<^bold>p\<^bold>r\<^bold>e\<^
   \<comment> \<open>A tag to hint automatic provers to try to prove this proof obligation\<close>
 lemma Premise_I: "P \<Longrightarrow> \<^bold>p\<^bold>r\<^bold>e\<^bold>m\<^bold>i\<^bold>s\<^bold>e P" unfolding Premise_def by simp
 lemma Premise_E: "\<^bold>p\<^bold>r\<^bold>e\<^bold>m\<^bold>i\<^bold>s\<^bold>e P \<Longrightarrow> P" unfolding Premise_def by simp
-lemma [elim,\<nu>elim]: "\<^bold>p\<^bold>r\<^bold>e\<^bold>m\<^bold>i\<^bold>s\<^bold>e P \<Longrightarrow> (P \<Longrightarrow> C) \<Longrightarrow> C" unfolding Premise_def by simp
+lemma [elim!,\<nu>elim]: "\<^bold>p\<^bold>r\<^bold>e\<^bold>m\<^bold>i\<^bold>s\<^bold>e P \<Longrightarrow> (P \<Longrightarrow> C) \<Longrightarrow> C" unfolding Premise_def by simp
 lemma Premise_Irew: "(P \<Longrightarrow> PROP C) \<equiv> (\<^bold>p\<^bold>r\<^bold>e\<^bold>m\<^bold>i\<^bold>s\<^bold>e P \<Longrightarrow> PROP C)" unfolding Premise_def by simp
 
 definition PremiseHOL :: "bool \<Rightarrow> bool" where "PremiseHOL x = x"
@@ -321,6 +321,7 @@ text \<open>The name `void` coincides that, when a procedure has no input argume
   the \<nu>-type for the input would exactly be @{term Void}. \<close>
 lemma [simp,intro]: "void \<in> Void" unfolding Void_def by simp
 lemma [simp,intro]: "Inhabited Void" unfolding Inhabited_def by auto
+lemma [elim!, \<nu>elim]: "Inhabited Void \<Longrightarrow> C \<Longrightarrow> C" .
 (*translations "a" <= "a \<^bold>a\<^bold>n\<^bold>d CONST Void"*)
 
 datatype 'a register = Register name_tag "'a::lrep"
@@ -389,7 +390,7 @@ lemma [intro]: "a \<in> A \<Longrightarrow> b \<in> B \<Longrightarrow> (a, b) \
 lemma [elim]: "ab \<in> (A and_ty B) \<Longrightarrow> (\<And>a b. ab = (a, b) \<Longrightarrow> a \<in> A \<Longrightarrow> b \<in> B \<Longrightarrow> C) \<Longrightarrow> C"
   unfolding AndTy_def And_def by (cases ab) simp
 lemma [intro]: "Inhabited A \<Longrightarrow> Inhabited B \<Longrightarrow> Inhabited (A and_ty B)" unfolding Inhabited_def AndTy_def And_def by auto
-lemma [elim,\<nu>elim]: "Inhabited (A and_ty B) \<Longrightarrow> (Inhabited A \<Longrightarrow> Inhabited B \<Longrightarrow> C) \<Longrightarrow> C" unfolding Inhabited_def by auto
+lemma [elim!,\<nu>elim]: "Inhabited (A and_ty B) \<Longrightarrow> (Inhabited A \<Longrightarrow> Inhabited B \<Longrightarrow> C) \<Longrightarrow> C" unfolding Inhabited_def by auto
 lemma [\<nu>intro]: "\<nu>Disposable A \<Longrightarrow> \<nu>Disposable B \<Longrightarrow> \<nu>Disposable (A and_ty B)"
   unfolding \<nu>Disposable_def by auto
 
@@ -410,7 +411,7 @@ lemma Stack_Delimiter_I[intro]: "a \<in> A \<Longrightarrow> b \<in> B \<Longrig
 lemma Stack_Delimiter_E[elim]: "ab \<in> (B \<heavy_comma> A) \<Longrightarrow> (\<And>a b. ab = (a,b) \<Longrightarrow> a \<in> A \<Longrightarrow> b \<in> B \<Longrightarrow> C) \<Longrightarrow> C" unfolding Stack_Delimiter_def by (cases ab) simp
 lemma [simp]: "Inhabited (U\<heavy_comma>V) \<longleftrightarrow> Inhabited U \<and> Inhabited V" unfolding Inhabited_def by auto
 lemma [intro]: "Inhabited U \<Longrightarrow> Inhabited V \<Longrightarrow> Inhabited (U\<heavy_comma>V)" unfolding Inhabited_def by auto
-lemma [elim,\<nu>elim]: "Inhabited (U\<heavy_comma>V) \<Longrightarrow> (Inhabited U \<Longrightarrow> Inhabited V \<Longrightarrow> PROP C) \<Longrightarrow> PROP C" unfolding Inhabited_def by auto
+lemma [elim!,\<nu>elim]: "Inhabited (U\<heavy_comma>V) \<Longrightarrow> (Inhabited U \<Longrightarrow> Inhabited V \<Longrightarrow> PROP C) \<Longrightarrow> PROP C" unfolding Inhabited_def by auto
 
 subsection \<open>Procedure construction context.\<close>
 
@@ -430,7 +431,7 @@ lemma [elim]: "c \<in> (X \<flower> G) \<Longrightarrow> (\<And>x g. c = Proc_Ct
 lemma [intro]: "x \<in> X \<Longrightarrow> g \<in> G \<Longrightarrow> Proc_Ctx x g \<in> (X \<flower> G)" unfolding Proc_CtxTy_def by auto
 lemma [simp]: "Inhabited (X \<flower> G) \<longleftrightarrow> Inhabited X \<and> Inhabited G"
   unfolding Proc_CtxTy_def Inhabited_def by auto
-lemma [elim,\<nu>elim]: "Inhabited (X \<flower> G) \<Longrightarrow> (Inhabited X \<Longrightarrow> Inhabited G \<Longrightarrow> C) \<Longrightarrow> C"
+lemma [elim!,\<nu>elim]: "Inhabited (X \<flower> G) \<Longrightarrow> (Inhabited X \<Longrightarrow> Inhabited G \<Longrightarrow> C) \<Longrightarrow> C"
   unfolding Proc_CtxTy_def Inhabited_def by auto
 lemma [intro]: "Inhabited X \<Longrightarrow> Inhabited G \<Longrightarrow> Inhabited (X \<flower> G)"
   unfolding Proc_CtxTy_def Inhabited_def by auto
@@ -445,7 +446,7 @@ lemma [simp]: "(Proc_Ctx s r) \<in> (T \<flower> U) \<equiv> s \<in> T \<and> r 
 lemma [\<nu>elim]: "c \<in> (T \<flower> U) \<Longrightarrow> (\<And>s r. c = (Proc_Ctx s r) \<Longrightarrow> s \<in> T \<Longrightarrow> r \<in> U \<Longrightarrow> C) \<Longrightarrow> C" by (cases c) auto
 lemma Proc_CtxTy_intro[intro]: "s \<in> T \<Longrightarrow> r \<in> U \<Longrightarrow> Proc_Ctx s r \<in> (T \<flower> U)" by (simp add: Proc_CtxTy_def)
 lemma [intro]: "Inhabited T \<Longrightarrow> Inhabited U \<Longrightarrow> Inhabited (T \<flower> U)" unfolding Inhabited_def by auto
-lemma [elim,\<nu>elim]: "Inhabited (T \<flower> U) \<Longrightarrow> (Inhabited T \<Longrightarrow> Inhabited U \<Longrightarrow> C) \<Longrightarrow> C" unfolding Inhabited_def by (auto elim: \<nu>elim)
+lemma [elim!,\<nu>elim]: "Inhabited (T \<flower> U) \<Longrightarrow> (Inhabited T \<Longrightarrow> Inhabited U \<Longrightarrow> C) \<Longrightarrow> C" unfolding Inhabited_def by (auto elim: \<nu>elim)
 
 subsection \<open>The \<nu>-system VM and Procedure construction structures\<close>
 
@@ -633,7 +634,7 @@ definition CurrentConstruction :: " ('a::lrep) state \<Rightarrow> 'a set \<Righ
 definition PendingConstruction :: " (('a::lrep) \<Rightarrow> ('b::lrep) state) \<Rightarrow> 'a state \<Rightarrow> 'b set \<Rightarrow> bool " ("\<^bold>p\<^bold>e\<^bold>n\<^bold>d\<^bold>i\<^bold>n\<^bold>g _ \<^bold>o\<^bold>n _ \<^bold>r\<^bold>e\<^bold>s\<^bold>u\<^bold>l\<^bold>t\<^bold>s \<^bold>i\<^bold>n/ _" [1000,1000,5] 4)
   where "PendingConstruction f s S \<longleftrightarrow> bind s f \<in> \<S> S"
 
-lemma [elim,\<nu>elim]: "CurrentConstruction s S \<Longrightarrow> (Inhabited S \<Longrightarrow> C) \<Longrightarrow> C" unfolding CurrentConstruction_def by auto
+lemma [elim!,\<nu>elim]: "CurrentConstruction s S \<Longrightarrow> (Inhabited S \<Longrightarrow> C) \<Longrightarrow> C" unfolding CurrentConstruction_def by auto
 
 definition CodeBlock :: " ('a::lrep) state \<Rightarrow> ('b::lrep) => 'b set \<Rightarrow> ('b \<Rightarrow> 'a state) \<Rightarrow> bool" where
   CodeBlock_def: "CodeBlock stat arg ty prog \<longleftrightarrow> (arg \<in> ty \<and> prog arg = stat \<and> stat \<noteq> SNeg)"
@@ -662,7 +663,7 @@ print_translation \<open>
   end
 \<close>
 
-lemma [elim,\<nu>elim]: "CodeBlock v arg ty prog \<Longrightarrow> (Inhabited ty \<Longrightarrow> C) \<Longrightarrow> C" unfolding CodeBlock_def by auto
+lemma [elim!,\<nu>elim]: "CodeBlock v arg ty prog \<Longrightarrow> (Inhabited ty \<Longrightarrow> C) \<Longrightarrow> C" unfolding CodeBlock_def by auto
 lemma CodeBlock_unabbrev: "CodeBlock v arg ty prog \<Longrightarrow> (v \<equiv> ProtectorI (prog arg))"
   unfolding CodeBlock_def ProtectorI_def by (rule eq_reflection) fast
 lemma CodeBlock_abbrev: "CodeBlock v arg ty prog \<Longrightarrow> ProtectorI (prog arg) \<equiv> v"
@@ -674,12 +675,14 @@ translations "Fact_sugar_ name P" == "CONST Fact (NAME name) P"
 lemma Fact_I: "P \<Longrightarrow> PROP Fact label P" unfolding Fact_def .
 lemma Fact_D: "\<^item> name : P \<Longrightarrow> P" unfolding Fact_def .
 
+
 definition FactCollection :: "prop \<Rightarrow> prop \<Rightarrow> prop \<Rightarrow> prop"
   where "FactCollection (PROP P) (PROP Q) (PROP S) \<equiv> (PROP P &&& PROP Q &&& PROP S)"
+    \<comment> \<open>P: star fact, Q: fact list, S: \<nu>current\<close>
 consts FactCollection_sugar :: "prop \<Rightarrow> prop \<Rightarrow> prop"  ("\<glowing_star> _/ \<^bold>a\<^bold>n\<^bold>d _" [4,3] 3)
-translations
+(* translations
   "Q" <= " CONST FactCollection (CONST NoFact) Q S"
-  "CONST FactCollection_sugar P Q" <= "CONST FactCollection P Q S"
+  "CONST FactCollection_sugar P Q" <= "CONST FactCollection P Q S" *)
 lemma FactCollection_imp: " (PROP FactCollection (PROP P) (PROP Q) (PROP S) \<Longrightarrow> PROP R) \<equiv> (PROP P \<Longrightarrow> PROP Q \<Longrightarrow> PROP S \<Longrightarrow> PROP R)"
   unfolding FactCollection_def conjunction_imp by rule
 lemma FactCollection_I: "PROP P \<Longrightarrow> PROP Q \<Longrightarrow> PROP S \<Longrightarrow> PROP  FactCollection (PROP P) (PROP Q) (PROP S)"
@@ -773,10 +776,12 @@ lemma declare_fact:
   "A \<Longrightarrow> (PROP P \<^bold>w\<^bold>i\<^bold>t\<^bold>h \<^bold>f\<^bold>a\<^bold>c\<^bold>t\<^bold>s: PROP FactCollection (PROP Q) (PROP L) (PROP S))
     \<Longrightarrow> (PROP P \<^bold>w\<^bold>i\<^bold>t\<^bold>h \<^bold>f\<^bold>a\<^bold>c\<^bold>t\<^bold>s: PROP FactCollection (PROP Q) (PROP Fact name A and_fact PROP L) (PROP S))"
   unfolding SpecTop_imp FactCollection_imp by (intro SpecTop_I FactCollection_I TrueI Fact_I AndFact_I NoFact)
-lemma intro_internal_fact:
-  "PROP A \<Longrightarrow> PROP FactCollection (PROP Q) (PROP L) (PROP S)
-    \<Longrightarrow> PROP FactCollection (PROP Q) (PROP L) (PROP A and_fact PROP S)"
-  unfolding SpecTop_imp FactCollection_imp by (intro SpecTop_I FactCollection_I TrueI Fact_I AndFact_I NoFact)
+
+lemma set_\<nu>current:
+  "(\<^bold>c\<^bold>u\<^bold>r\<^bold>r\<^bold>e\<^bold>n\<^bold>t s \<^bold>r\<^bold>e\<^bold>s\<^bold>u\<^bold>l\<^bold>t\<^bold>s \<^bold>i\<^bold>n T \<^bold>w\<^bold>i\<^bold>t\<^bold>h \<^bold>f\<^bold>a\<^bold>c\<^bold>t\<^bold>s: PROP FactCollection (PROP Q) (PROP L) (PROP S))
+    \<Longrightarrow> (\<^bold>c\<^bold>u\<^bold>r\<^bold>r\<^bold>e\<^bold>n\<^bold>t s \<^bold>r\<^bold>e\<^bold>s\<^bold>u\<^bold>l\<^bold>t\<^bold>s \<^bold>i\<^bold>n T \<^bold>w\<^bold>i\<^bold>t\<^bold>h \<^bold>f\<^bold>a\<^bold>c\<^bold>t\<^bold>s: PROP FactCollection (PROP Q) (PROP L) (Trueprop (Inhabited T)))"
+  unfolding SpecTop_imp FactCollection_imp by (intro SpecTop_I FactCollection_I TrueI Fact_I AndFact_I NoFact) auto
+
 lemma clean_user_facts:
   "(PROP P \<^bold>w\<^bold>i\<^bold>t\<^bold>h \<^bold>f\<^bold>a\<^bold>c\<^bold>t\<^bold>s: PROP FactCollection (PROP Q) (PROP L) (PROP S)) \<Longrightarrow>
     (PROP P \<^bold>w\<^bold>i\<^bold>t\<^bold>h \<^bold>f\<^bold>a\<^bold>c\<^bold>t\<^bold>s: PROP FactCollection NoFact NoFact (PROP S))"
@@ -878,8 +883,6 @@ lemma [\<nu>intro]: "\<^bold>p\<^bold>r\<^bold>e\<^bold>m\<^bold>i\<^bold>s\<^bo
 lemma [\<nu>intro]: "\<^bold>c\<^bold>a\<^bold>s\<^bold>t A \<longmapsto> B \<^bold>m\<^bold>e\<^bold>a\<^bold>n\<^bold>w\<^bold>h\<^bold>i\<^bold>l\<^bold>e P \<Longrightarrow> \<^bold>c\<^bold>a\<^bold>s\<^bold>t \<S_S> A \<longmapsto> \<S_S> B \<^bold>m\<^bold>e\<^bold>a\<^bold>n\<^bold>w\<^bold>h\<^bold>i\<^bold>l\<^bold>e P" by blast
 lemma [\<nu>intro]: "\<^bold>c\<^bold>a\<^bold>s\<^bold>t A \<longmapsto> A' \<^bold>m\<^bold>e\<^bold>a\<^bold>n\<^bold>w\<^bold>h\<^bold>i\<^bold>l\<^bold>e P1 \<Longrightarrow> \<^bold>c\<^bold>a\<^bold>s\<^bold>t B \<longmapsto> B' \<^bold>m\<^bold>e\<^bold>a\<^bold>n\<^bold>w\<^bold>h\<^bold>i\<^bold>l\<^bold>e P2 \<Longrightarrow> \<^bold>c\<^bold>a\<^bold>s\<^bold>t (A\<heavy_comma>B) \<longmapsto> (A'\<heavy_comma>B') \<^bold>m\<^bold>e\<^bold>a\<^bold>n\<^bold>w\<^bold>h\<^bold>i\<^bold>l\<^bold>e P1 \<and> P2" by blast
 lemma LooseState_Cast[\<nu>intro]: "\<^bold>c\<^bold>a\<^bold>s\<^bold>t A \<longmapsto> B \<Longrightarrow> \<^bold>c\<^bold>a\<^bold>s\<^bold>t \<S> A \<longmapsto> \<S> B" unfolding \<nu>def Cast_def by auto
-lemma [\<nu>intro]: "\<^bold>c\<^bold>a\<^bold>s\<^bold>t A \<longmapsto> A' \<^bold>m\<^bold>e\<^bold>a\<^bold>n\<^bold>w\<^bold>h\<^bold>i\<^bold>l\<^bold>e P \<Longrightarrow> \<^bold>c\<^bold>a\<^bold>s\<^bold>t B \<longmapsto> B' \<^bold>m\<^bold>e\<^bold>a\<^bold>n\<^bold>w\<^bold>h\<^bold>i\<^bold>l\<^bold>e Q \<Longrightarrow> \<^bold>c\<^bold>a\<^bold>s\<^bold>t (A\<heavy_comma>B) \<longmapsto> (A'\<heavy_comma>B') \<^bold>m\<^bold>e\<^bold>a\<^bold>n\<^bold>w\<^bold>h\<^bold>i\<^bold>l\<^bold>e P \<and>Q"
-  unfolding Cast_def by auto
 lemma [\<nu>intro]: "\<^bold>c\<^bold>a\<^bold>s\<^bold>t A \<longmapsto> A' \<^bold>m\<^bold>e\<^bold>a\<^bold>n\<^bold>w\<^bold>h\<^bold>i\<^bold>l\<^bold>e P \<Longrightarrow> \<^bold>c\<^bold>a\<^bold>s\<^bold>t B \<longmapsto> B' \<^bold>m\<^bold>e\<^bold>a\<^bold>n\<^bold>w\<^bold>h\<^bold>i\<^bold>l\<^bold>e Q \<Longrightarrow> \<^bold>c\<^bold>a\<^bold>s\<^bold>t (A \<flower> B) \<longmapsto> (A' \<flower> B') \<^bold>m\<^bold>e\<^bold>a\<^bold>n\<^bold>w\<^bold>h\<^bold>i\<^bold>l\<^bold>e P \<and> Q"
   unfolding Cast_def by auto
 lemma [\<nu>intro]: "\<^bold>c\<^bold>a\<^bold>s\<^bold>t A \<longmapsto> A' \<^bold>m\<^bold>e\<^bold>a\<^bold>n\<^bold>w\<^bold>h\<^bold>i\<^bold>l\<^bold>e P \<Longrightarrow> \<^bold>c\<^bold>a\<^bold>s\<^bold>t B \<longmapsto> B' \<^bold>m\<^bold>e\<^bold>a\<^bold>n\<^bold>w\<^bold>h\<^bold>i\<^bold>l\<^bold>e Q \<Longrightarrow> \<^bold>c\<^bold>a\<^bold>s\<^bold>t (A and_ty B) \<longmapsto> (A' and_ty B') \<^bold>m\<^bold>e\<^bold>a\<^bold>n\<^bold>w\<^bold>h\<^bold>i\<^bold>l\<^bold>e P \<and> Q"
@@ -889,6 +892,9 @@ theorem apply_cast: "(\<^bold>c\<^bold>u\<^bold>r\<^bold>r\<^bold>e\<^bold>n\<^b
   unfolding Procedure_def CurrentConstruction_def PendingConstruction_def bind_def SpecTop_imp by (auto 4 6)
 theorem cast: "\<^bold>c\<^bold>u\<^bold>r\<^bold>r\<^bold>e\<^bold>n\<^bold>t blk \<^bold>r\<^bold>e\<^bold>s\<^bold>u\<^bold>l\<^bold>t\<^bold>s \<^bold>i\<^bold>n T \<Longrightarrow> \<^bold>c\<^bold>a\<^bold>s\<^bold>t T \<longmapsto> T' \<^bold>m\<^bold>e\<^bold>a\<^bold>n\<^bold>w\<^bold>h\<^bold>i\<^bold>l\<^bold>e P \<Longrightarrow> \<^bold>c\<^bold>u\<^bold>r\<^bold>r\<^bold>e\<^bold>n\<^bold>t blk \<^bold>r\<^bold>e\<^bold>s\<^bold>u\<^bold>l\<^bold>t\<^bold>s \<^bold>i\<^bold>n T' "
   for T' :: "('a::lrep) set" unfolding Cast_def CurrentConstruction_def by auto
+
+theorem proc_cast': "\<^bold>p\<^bold>r\<^bold>o\<^bold>c f \<blangle> A \<longmapsto> B \<brangle> \<Longrightarrow> \<^bold>c\<^bold>a\<^bold>s\<^bold>t A' \<longmapsto> A \<^bold>m\<^bold>e\<^bold>a\<^bold>n\<^bold>w\<^bold>h\<^bold>i\<^bold>l\<^bold>e P \<Longrightarrow> \<^bold>c\<^bold>a\<^bold>s\<^bold>t B \<longmapsto> B' \<^bold>m\<^bold>e\<^bold>a\<^bold>n\<^bold>w\<^bold>h\<^bold>i\<^bold>l\<^bold>e Q \<Longrightarrow> \<^bold>p\<^bold>r\<^bold>o\<^bold>c f \<blangle> A' \<longmapsto> B' \<brangle>"
+  unfolding Procedure_def Cast_def by (auto 0 3)
 
 subsubsection \<open>Conversion\<close>
 
